Add some lemmas in preparation for `exp_eq` completeness

meta-theory/pure_ctxt_equivScript.sml
@@ -1,11 +1,14 @@
 
 open HolKernel Parse boolLib bossLib term_tactic;
 open arithmeticTheory listTheory stringTheory alistTheory optionTheory
-     ltreeTheory llistTheory bagTheory pairTheory pred_setTheory;
-open pure_evalTheory pure_exp_lemmasTheory pure_expTheory pure_congruenceTheory
-
+     pairTheory pred_setTheory;
+open pure_expTheory pure_exp_lemmasTheory
+     pure_exp_relTheory pure_congruenceTheory
 
 val _ = new_theory "pure_ctxt_equiv";
+
+
+(******************** Basic definitions ********************)
 
 Datatype:
   ctxt = Hole
@@ -28,6 +31,47 @@ Definition plug_def:
   plug (LetrecL xs1 (f,h) xs2 x) n = Letrec (xs1 ++ [(f,plug h n)] ++ xs2) x ∧
   plug (LetrecR xs h) n = Letrec xs (plug h n)
 End
+
+Definition plug_ctxt_def:
+  plug_ctxt Hole n = n ∧
+  plug_ctxt (Prim op xs1 h xs2) n = Prim op xs1 (plug_ctxt h n) xs2 ∧
+  plug_ctxt (AppL h y) n = AppL (plug_ctxt h n) y ∧
+  plug_ctxt (AppR x h) n = AppR x (plug_ctxt h n) ∧
+  plug_ctxt (Lam v h) n = Lam v (plug_ctxt h n) ∧
+  plug_ctxt (LetrecL xs1 (f,h) xs2 x) n = LetrecL xs1 (f, plug_ctxt h n) xs2 x ∧
+  plug_ctxt (LetrecR xs h) n = LetrecR xs (plug_ctxt h n)
+End
+
+Definition AppLs_def:
+  AppLs c [] = c ∧
+  AppLs c (e::es) = AppLs (AppL c e) es
+End
+
+Definition LamsC_def:
+  LamsC [] c = c :ctxt ∧
+  LamsC (v::vs) c = Lam v (LamsC vs c)
+End
+
+
+(******************** Lemmas ********************)
+
+Theorem plug_AppLs:
+  ∀l c e. plug (AppLs c l) e = Apps (plug c e) l
+Proof
+  Induct >> rw[AppLs_def, Apps_def, plug_def]
+QED
+
+Theorem plug_LamsC:
+  ∀l c e. plug (LamsC l c) e = Lams l (plug c e)
+Proof
+  Induct >> rw[LamsC_def, Lams_def, plug_def]
+QED
+
+Theorem plug_plug_ctxt:
+  ∀c1 c2 e. plug (plug_ctxt c1 c2) e = plug c1 (plug c2 e)
+Proof
+  recInduct plug_ctxt_ind >> rw[plug_def, plug_ctxt_def]
+QED
 
 Theorem exp_equiv_plug:
   ∀h x y. x ≅ y ⇒ plug h x ≅ plug h y
@@ -58,23 +102,37 @@ Proof
     )
 QED
 
-(****************************************)
-
-Definition plug_ctxt_def:
-  plug_ctxt Hole n = n ∧
-  plug_ctxt (Prim op xs1 h xs2) n = Prim op xs1 (plug_ctxt h n) xs2 ∧
-  plug_ctxt (AppL h y) n = AppL (plug_ctxt h n) y ∧
-  plug_ctxt (AppR x h) n = AppR x (plug_ctxt h n) ∧
-  plug_ctxt (Lam v h) n = Lam v (plug_ctxt h n) ∧
-  plug_ctxt (LetrecL xs1 (f,h) xs2 x) n = LetrecL xs1 (f, plug_ctxt h n) xs2 x ∧
-  plug_ctxt (LetrecR xs h) n = LetrecR xs (plug_ctxt h n)
-End
-
-Theorem plug_plug_ctxt:
-  ∀c1 c2 e. plug (plug_ctxt c1 c2) e = plug c1 (plug c2 e)
+Theorem freevars_plug_eq:
+  ∀ctxt e1 e2.
+    freevars e1 = freevars e2
+  ⇒ freevars (plug ctxt e1) = freevars (plug ctxt e2)
 Proof
-  recInduct plug_ctxt_ind >> rw[plug_def, plug_ctxt_def]
+  recInduct plug_ind >> rw[plug_def]
+  >- (AP_THM_TAC >> ntac 2 AP_TERM_TAC >> first_x_assum irule >> simp[])
+  >- (AP_THM_TAC >> AP_TERM_TAC >> first_x_assum irule >> simp[])
+  >- (AP_TERM_TAC >> first_x_assum irule >> simp[])
+  >- (AP_THM_TAC >> AP_TERM_TAC >> first_x_assum irule >> simp[])
+  >- (
+    AP_THM_TAC >> ntac 2 AP_TERM_TAC >> AP_THM_TAC >>
+    ntac 2 AP_TERM_TAC >> first_x_assum irule >> simp[]
+    )
+  >- (
+    AP_THM_TAC >> AP_TERM_TAC >> AP_THM_TAC >> AP_TERM_TAC >>
+    first_x_assum irule >> simp[]
+    )
 QED
+
+Triviality app_bisimilarity_plug:
+  ∀c x y. x ≃ y ∧ closed (plug c x) ⇒ plug c x ≃ plug c y
+Proof
+  rw[app_bisimilarity_eq]
+  >- (irule exp_equiv_plug >> simp[])
+  >- (
+    gvs[closed_def] >>
+    qspecl_then [`c`,`x`,`y`] assume_tac freevars_plug_eq >> gvs[]
+    )
+QED
+
 
 (****************************************)
 
